Pcc116Code/Aula13.lean
@@ -1,0 +1,5 @@
+-- Aula 13: λ-cálculo tipado simples. 
+
+import Mathlib.Data.Nat.Defs 
+
+
